more progress on the progress theorem

theories/type_progress.v
@@ -194,6 +194,9 @@ Definition not_lf_br (es: seq administrative_instruction) (n: nat) :=
 Definition not_lf_return (es: seq administrative_instruction) (n: nat) :=
   forall (lh: lholed n), lfill lh [::AI_basic BI_return] <> es.
 
+Definition not_lf_return_invoke (es: seq administrative_instruction) (n: nat) :=
+  forall (lh: lholed n) (a: funcaddr), lfill lh [::AI_return_invoke a] <> es.
+
 Lemma nlfbr_right: forall es n es',
     not_lf_br (es ++ es') n ->
     not_lf_br es n.
@@ -211,6 +214,17 @@ Lemma nlfret_right: forall es n es',
 Proof.
   unfold not_lf_return.
   move => es n es' HNLF lh HContra.
+  subst es.
+  rewrite -lfill_push_back_es in HNLF.
+  by eapply HNLF.
+Qed.
+
+Lemma nlfretinv_right: forall es n es',
+    not_lf_return_invoke (es ++ es') n ->
+    not_lf_return_invoke es n.
+Proof.
+  unfold not_lf_return_invoke.
+  move => es n es' HNLF lh a HContra.
   subst es.
   rewrite -lfill_push_back_es in HNLF.
   by eapply HNLF.
@@ -235,6 +249,18 @@ Lemma nlfret_left: forall es n cs vcs,
 Proof.
   unfold not_lf_return.
   move => es n vcs cs -> IH lh ?.
+  subst es.
+  erewrite <- lfill_push_front_vs in IH; eauto.
+  by eapply IH.
+Qed.
+
+Lemma nlfretinv_left: forall es n cs vcs,
+    cs = v_to_e_list vcs ->
+    not_lf_return_invoke (cs ++ es) n ->
+    not_lf_return_invoke es n.
+Proof.
+  unfold not_lf_return.
+  move => es n vcs cs -> IH lh a ?.
   subst es.
   erewrite <- lfill_push_front_vs in IH; eauto.
   by eapply IH.
@@ -272,10 +298,11 @@ Lemma t_progress_be: forall C bes ts1 ts2 vcs lab ret s f hs,
     map typeof vcs = ts1 ->
     not_lf_br (to_e_list bes) 0 ->
     not_lf_return (to_e_list bes) 0 ->
+    not_lf_return_invoke (to_e_list bes) 0 ->
     const_list (to_e_list bes) \/
     exists s' f' es' hs', reduce hs s f (v_to_e_list vcs ++ to_e_list bes) hs' s' f' es'.
 Proof.
-  move => C bes ts1 ts2 vcs lab ret s f hs HST HIT HType HConstType HNBI_br HNRet.
+  move => C bes ts1 ts2 vcs lab ret s f hs HST HIT HType HConstType HNBI_br HNRet HNRetInv.
   generalize dependent vcs.
   gen_ind HType; try by left.
   - (* Unop *)
@@ -585,19 +612,23 @@ Proof.
     subst.
     rewrite to_e_list_cat in HNBI_br.
     rewrite to_e_list_cat in HNRet.
+    rewrite to_e_list_cat in HNRetInv.
     clear H.
     edestruct IHHType1; eauto.
     { by eapply nlfbr_right; eauto. }
     { by eapply nlfret_right; eauto. }
+    { by eapply nlfretinv_right; eauto. }
     + (* Const *)
       apply const_es_exists in H. destruct H as [cs HConst].
       apply b_e_elim in HConst. destruct HConst. subst.
       rewrite e_b_inverse in HNRet; last by apply const_list_is_basic; apply v_to_e_const.
       rewrite e_b_inverse in HNBI_br; last by apply const_list_is_basic; apply v_to_e_const.
+      rewrite e_b_inverse in HNRetInv; last by apply const_list_is_basic; apply v_to_e_const.
       apply Const_list_typing in HType1. subst.
       edestruct IHHType2; eauto.
       { by eapply nlfbr_left; try apply v_to_e_const; eauto. }
       { by eapply nlfret_left; try apply v_to_e_const; eauto. }
+      { by eapply nlfretinv_left; try apply v_to_e_const; eauto. }
       { by rewrite -map_cat. }
       * left. rewrite to_e_list_cat. apply const_list_concat => //.
         by rewrite e_b_inverse => //; apply v_to_e_const.
@@ -637,6 +668,9 @@ Definition br_reduce (es: seq administrative_instruction) :=
 Definition return_reduce (es: seq administrative_instruction) :=
   exists n (lh: lholed n), lfill lh [::AI_basic BI_return] = es.
 
+Definition return_invoke_reduce (es: seq administrative_instruction) :=
+  exists a n (lh: lholed n), lfill lh [::AI_return_invoke a] = es.
+
 (** [br_reduce] is decidable. **)
 Lemma br_reduce_decidable : forall es, decidable (br_reduce es).
   move => es.
@@ -661,7 +695,20 @@ Proof.
     move => [n [lh Heq]].
     by apply (He n lh).
 Qed.
-  
+
+(** [return_invoke_reduce] is decidable. **)
+Lemma return_invoke_reduce_decidable : forall es, decidable (return_invoke_reduce es).
+Proof.
+  (* move => es a.
+  destruct (lfill_factorise (fun _ => AI_return_invoke a) es) as [[n [lh Heq]] | He].
+  - subst es.
+    left.
+    by repeat eexists.
+  - right.
+    move => [a' [n [lh Heq]]].
+    by apply (He n lh). *)
+Admitted.  (* may have to adjust lfill_factorise *)
+
 Lemma br_reduce_label_length: forall n k (lh: lholed n) es s C ts2,
     lfill lh [::AI_basic (BI_br (n + k))] = es ->
     e_typing s C es (Tf [::] ts2) ->
@@ -701,6 +748,24 @@ Proof.
     invert_e_typing'.
     by assert (tc_return (upd_label C ([::ts_label] ++ tc_label C)) <> None); first by eapply IH; eauto.
 Qed.
+
+Lemma return_invoke_reduce_return_some: forall n (lh: lholed n) a es s C ts2,
+    lfill lh [::AI_return_invoke a] = es ->
+    e_typing s C es (Tf [::] ts2) ->
+    tc_return C <> None.
+Proof.
+  move => n.
+  elim.
+  - move => vs es a es' s C ts <- /=Hetype.
+    rewrite -cat1s in Hetype.
+    invert_e_typing'.
+    admit. (* needs inversion lemma for return_invoke *)
+    (* by rewrite H2_return. *)
+  - move => k vs n0 es lh IH es' a es'' s C ts <- /=Hetype.
+    rewrite -cat1s in Hetype.
+    invert_e_typing'.
+    by assert (tc_return (upd_label C ([::ts_label] ++ tc_label C)) <> None); first by eapply IH; eauto.
+Admitted.
 
 Lemma br_reduce_extract_vs: forall n k (lh: lholed n) es s C ts ts2,
     lfill lh [::AI_basic (BI_br (n + k))] = es ->
@@ -821,6 +886,16 @@ Proof.
   by eapply return_reduce_return_some in H1; eauto.
 Qed.
 
+Lemma s_typing_lf_return_invoke: forall s f es ts,
+    s_typing s None f es ts ->
+    (forall n, not_lf_return_invoke es n).
+Proof.
+  unfold not_lf_return_invoke.
+  move => s f es ts HType n lh a HContra.
+  inversion HType; subst.
+  by eapply return_invoke_reduce_return_some in H1; eauto.
+Qed.
+
 Axiom host_application_exists: forall hs s tf hf vcs,
     exists hs' res, host_application hs s tf hf vcs hs' res.
 
@@ -833,6 +908,7 @@ Lemma t_progress_e: forall s C C' f vcs es tf ts1 ts2 lab ret hs,
     store_typing s ->
     (forall n (lh: lholed n) k, lfill lh [::AI_basic (BI_br k)] = es -> k < n) ->
     (forall n, not_lf_return es n) ->
+    (forall n, not_lf_return_invoke es n) ->
     terminal_form (v_to_e_list vcs ++ es) \/
     exists s' f' es' hs', reduce hs s f (v_to_e_list vcs ++ es) hs' s' f' es'.
 Proof.
@@ -849,19 +925,21 @@ Proof.
               store_typing s ->
               (forall n (lh: lholed n) k, lfill lh [::AI_basic (BI_br k)] = es -> k < n) ->
               (forall n, not_lf_return es n) ->
+              (forall n, not_lf_return_invoke es n) ->
               terminal_form (v_to_e_list vcs ++ es) \/
               exists s' f' es' hs', reduce hs s f (v_to_e_list vcs ++ es) hs' s' f' es')
     (P0 := fun s rs f es ts (_ : s_typing s rs f es ts) => forall hs,
               store_typing s ->
               (forall n (lh: lholed n) k, lfill lh [::AI_basic (BI_br k)] = es -> k < n) ->
               (forall n, not_lf_return es n) ->
+              (forall n, not_lf_return_invoke es n) ->
               (const_list es /\ length es = length ts) \/
               es = [::AI_trap] \/
               exists s' f' es' hs', reduce hs s f es hs' s' f' es'); clear HType s C es tf.
    
   - (* AI_basic *)
     move => s C bes tf HType.
-    move => f C' vcs ts1 ts2 lab ret hs HTF HContext HInst HConstType HST HBI_brDepth HNRet.
+    move => f C' vcs ts1 ts2 lab ret hs HTF HContext HInst HConstType HST HBI_brDepth HNRet HNRetInv.
     subst.
     eapply t_progress_be in HType; try instantiate (1 := vs) in HType; try by eauto.
     destruct HType as [HType | [s' [vs' [es' [hs' HType]]]]].
@@ -874,7 +952,7 @@ Proof.
       by apply HBI_brDepth in HContra.
   - (* Composition *)
     move => s C es e t1s t2s t3s HType1 IHHType1 HType2 IHHType2.
-    move => f C' vcs ts1 ts2 lab ret hs HTF HContext HInst HConstType HST HBI_brDepth HNRet.
+    move => f C' vcs ts1 ts2 lab ret hs HTF HContext HInst HConstType HST HBI_brDepth HNRet HNRetInv.
     inversion HTF; subst.
     edestruct IHHType1; eauto.
     { move => n lh k HLF.
@@ -884,6 +962,8 @@ Proof.
     }
     { move => n.
       eapply nlfret_right. by apply HNRet. }
+    { move => n.
+      eapply nlfretinv_right. by apply HNRetInv. }
     + (* Terminal *)
       unfold terminal_form in H. destruct H.
       * (* Const *)
@@ -899,9 +979,8 @@ Proof.
           rewrite - HLF.
           by apply lfill_push_front_vs.
         }
-        { move => n.
-          eapply nlfret_left; by eauto.
-        }
+        { move => n. eapply nlfret_left; by eauto. }
+        { move => n. eapply nlfretinv_left; by eauto. }
         -- (* Terminal *)
           unfold terminal_form in H. destruct H.
           ++ left. unfold terminal_form. left.
@@ -935,7 +1014,7 @@ Proof.
       * done.
   - (* Weakening *)
     move => s C es ts t1s t2s HType IHHType.
-    move => f C' vcs ts1 ts2 lab ret hs' HTF HContext HInst HConstType HST HBI_brDepth HNRet.
+    move => f C' vcs ts1 ts2 lab ret hs' HTF HContext HInst HConstType HST HBI_brDepth HNRet HNRetInv.
     inversion HTF; subst.
     symmetry in H0. apply cat_split in H0. destruct H0 as [HCT1 HCT2].
     rewrite - map_take in HCT1.
@@ -982,7 +1061,7 @@ Proof.
     by apply v_to_e_const.
   - (* Local *)
     move => s C n f0 es ts HType IHHType HLength.
-    move => f C' vcs ts1 ts2 lab ret hs HTF HContext HInst HConstType HST HBI_brDepth HNRet.
+    move => f C' vcs ts1 ts2 lab ret hs HTF HContext HInst HConstType HST HBI_brDepth HNRet HNRetInv.
     inversion HTF; subst; clear HTF.
     symmetry in H0.
     invert_typeof_vcs.
@@ -999,6 +1078,18 @@ Proof.
       eapply rs_return; eauto.
       by [].
     }
+    destruct (return_invoke_reduce_decidable es) as [HEMT' | HEMF']. (* not sure what HEMT stands for *)
+    { inversion HType; subst.
+      unfold return_invoke_reduce in HEMT'.
+      destruct HEMT' as [a [n [lh HLF]]].
+      (* eapply return_invoke_reduce_extract_vs in HLF; eauto.
+      instantiate (1 := ts2) in HLF.
+      destruct HLF as [cs [lh' [HConst [HLF2 HLength]]]].
+      repeat eexists.
+      apply r_simple.
+      eapply rs_return; eauto.
+      by []. *) admit.
+    }
     edestruct IHHType as [ | [ | ]]; eauto.
     {
       move => n lh k HLF.
@@ -1006,7 +1097,11 @@ Proof.
     }
     { unfold return_reduce in HEMF. unfold not_lf_return.
       move => n lh HContra.
-      apply HEMF. by eauto.
+      by apply HEMF; eauto.
+    }
+    { unfold return_invoke_reduce in HEMF'.
+      move => n lh a HContra.
+      by apply HEMF'; eauto.
     }
     + (* Const *)
       destruct H.
@@ -1046,9 +1141,15 @@ Proof.
         repeat eexists.
         eapply r_invoke_host_diverge; eauto.
         repeat rewrite length_is_size. by apply size_map.
+  - (* Return invoke *) {
+    move => s a C cl ts ts' t1s t2s HNth HType Hret.
+    move => f C' vcs ts1 ts2 lab ret hs HTF HContext HInst HConstType HST HBI_brDepth HNRet HNRetInv.
+    unfold not_lf_return_invoke in HNRetInv.
+    specialize HNRetInv with 0 (LH_base [::] [::]) a => //=HNRetInv. }
+
   - (* AI_label *)
-    move => s C e0s es ts t2s n HType1 IHHType1 HType2 IHHType2 HLength.
-    move => f C' vcs ts1 ts2 lab ret hs HTF HContext HInst HConstType HST HBI_brDepth HNRet.
+    move => s C e0s es ts t2s n HType1 IHHType1 HType2 IHHType2 Hlen.
+    move => f C' vcs ts1 ts2 lab ret hs HTF HContext HInst HConstType HST HBI_brDepth HNRet HNRetInv.
     inversion HTF; subst.
     symmetry in H0. invert_typeof_vcs.
     rewrite upd_label_overwrite in HType2. simpl in HType2.
@@ -1086,6 +1187,13 @@ Proof.
       instantiate (1 := LH_rec [::] (length ts) e0s lh [::]) => /=.
       by rewrite HContra.
     }
+    { unfold not_lf_return_invoke.
+      move => n lh a HContra.
+      unfold not_lf_return_invoke in HNRetInv.
+      eapply HNRetInv.
+      instantiate (2 := LH_rec [::] (length ts) e0s lh [::]) => /=.
+      by erewrite HContra.
+    }
     + (* Terminal *)
       apply terminal_form_v_e in H.
       unfold terminal_form in H. destruct H.
@@ -1109,7 +1217,7 @@ Proof.
       instantiate (1 := LH_rec nil (length ts) e0s (LH_base nil nil) nil).
       all: simpl; try by rewrite cats0.
   - (* s_typing *)
-    move => s f es rs ts C C0 HFT HContext HType IHHType HRetType hs HST HBI_brDepth HNRet.
+    move => s f es rs ts C C0 HFT HContext HType IHHType HRetType hs HST HBI_brDepth HNRet HNRetInv.
     inversion HFT.
     subst.
     edestruct IHHType; eauto.
@@ -1119,6 +1227,7 @@ Proof.
       rewrite E cats0. simpl.
       by fold_upd_context. }
     { by instantiate (1 := [::]). }
+
     + unfold terminal_form in H0. destruct H0.
       * (* Const *)
         left. split => //.
@@ -1132,7 +1241,7 @@ Proof.
         right. by left.
     + (* reduce *)
       simpl in H0. right. right. by eauto.
-Qed.
+Admitted.
 
 Theorem t_progress: forall s f es ts hs,
     config_typing s f es ts ->
@@ -1152,6 +1261,7 @@ Proof.
     by destruct C1.
   - by eapply s_typing_lf_br; eauto.
   - by eapply s_typing_lf_return; eauto.
+  - by eapply s_typing_lf_return_invoke; eauto.
 Qed.
 
 End Host.
